Added other type constructors

comp_expr.v
@@ -3,8 +3,8 @@ Require Import util.
 Require Import meta_term.
 Require Import meta_subst.
  
- Set Implicit Arguments.
- Inductive tp' ψ (δ:world):=
+Set Implicit Arguments.
+Inductive tp' ψ (δ:world):=
   | m_tp : mtype δ -> tp' ψ δ
   | arr : tp' ψ δ -> tp' ψ δ -> tp' ψ δ
   | pi : forall δ', δ↪δ' -> mtype δ -> tp' ψ δ' -> tp' ψ δ
@@ -12,22 +12,18 @@ Require Import meta_subst.
   | unit : tp' ψ δ
   | prod : tp' ψ δ -> tp' ψ δ -> tp' ψ δ
   | sum : tp' ψ δ -> tp' ψ δ -> tp' ψ δ
-(*  | mu : forall δ' ψ', star (fun δ1 δ2 => (mtype δ1)*(δ1↪δ2)) δ δ'
-         ->  ψ↪ψ'
-         -> tp' ψ' δ'
-         -> tp' ψ δ *)
   | tvar : name ψ -> tp' ψ δ
   | tapp : tp' ψ δ -> meta_term δ -> tp' ψ δ
   | eq_constraint : meta_term δ -> meta_term δ -> tp' ψ δ -> tp' ψ δ
- .
+  | mu : forall ψ', ψ↪ψ' -> tp' ψ' δ -> tp' ψ δ
+  | mlamt : forall δ', δ↪δ' -> mtype δ -> tp' ψ δ' -> tp' ψ δ
+.
 
- Definition tp δ := tp' ∅ δ.
- Unset Implicit Arguments.
- Definition m_tp' {δ} := @m_tp ∅ δ : mtype δ -> tp δ.
- Coercion m_tp' : mtype >-> tp.
+Definition tp δ := tp' ∅ δ.
+Definition m_tp' {δ} := @m_tp ∅ δ : mtype δ -> tp δ.
+Coercion m_tp' : mtype >-> tp.
 
-
- Inductive synth_exp (δ γ:world) : Set :=
+Inductive synth_exp (δ γ:world) : Set :=
   | var : name γ -> synth_exp δ γ
   | app :  synth_exp δ γ -> checked_exp δ γ -> synth_exp δ γ
   | mapp : synth_exp δ γ -> meta_term δ -> synth_exp δ γ
@@ -49,16 +45,5 @@ Require Import meta_subst.
   | tt : checked_exp δ γ
  with branch (δ γ:world) : Set :=
   | br : forall δi, meta_term δi -> msubst δ δi -> checked_exp δi γ -> branch δ γ.
- Coercion synth : synth_exp >-> checked_exp.
- Implicit Arguments var.
- Implicit Arguments app.
- Implicit Arguments mapp.
- Implicit Arguments coercion.
- Implicit Arguments synth.
- Implicit Arguments meta.
- Implicit Arguments fn.
- Implicit Arguments mlam.
- Implicit Arguments case_i.
- Implicit Arguments case_c.
- Implicit Arguments rec.
- Implicit Arguments br.
+
+Coercion synth : synth_exp >-> checked_exp.
